cedar-lean/Cedar/Thm/SymCC/Env/Soundness.lean
@@ -17,6 +17,7 @@
 import Cedar.Thm.Validation.Typechecker.Types
 import Cedar.Thm.SymCC.Concretizer
 import Cedar.SymCC.Concretizer
+import Cedar.SymCC.Symbolizer
 import Cedar.SymCC.Env
 
 /-!
@@ -30,10 +31,95 @@ open Cedar.Spec
 open Cedar.SymCC
 open Cedar.Validation
 
+/--
+`Value.symbolize?` is total on well-typed values,
+and the resulting term is a well-formed literal
+-/
+theorem value_symbolize?_same
+  {Γ : TypeEnv} {v : Value} {ty : CedarType}
+  (hwf : Γ.WellFormed)
+  (hwf_ty : ty.WellFormed Γ)
+  (hwt : InstanceOfType Γ v ty) :
+  ∃ t,
+    v.symbolize? ty = .some t ∧
+    v ∼ t
+:= by
+  cases hwt with
+  | instance_of_bool
+  | instance_of_string
+  | instance_of_entity
+  | instance_of_ext
+  | instance_of_int =>
+    simp [
+      Value.symbolize?, Prim.symbolize,
+      Same.same, SameValues,
+      Term.value?, TermPrim.value?, BitVec.int64?,
+    ]
+  | instance_of_set s sty hwt =>
+    simp [Value.symbolize?]
+    sorry
+  | instance_of_record rec =>
+    sorry
+
+theorem env_symbolize?_same_request
+  {Γ : TypeEnv} {env : Env}
+  (hinst : InstanceOfWellFormedEnvironment env.request env.entities Γ) :
+  env.request ∼ ((SymEnv.ofEnv Γ).interpret (env.symbolize? Γ)).request
+:= by
+  have hwf := hinst.wf_env
+  simp only [
+    SymEnv.interpret,
+    Env.symbolize?,
+    SymEnv.ofEnv,
+    SymRequest.ofRequestType,
+    SymRequest.interpret,
+    Request.symbolize?,
+    Value.symbolize?,
+    Prim.symbolize,
+  ]
+  and_intros
+  all_goals
+    simp only [Term.interpret]
+  -- Actions match
+  · have ⟨_, ⟨_, h, _, _⟩, _⟩ := hinst
+    simp [h]
+  -- Same context after interpretation
+  · have hwf_ctx_ty : (CedarType.record Γ.reqty.context).WellFormed Γ := by
+      have ⟨_, _, _, h⟩ := wf_env_implies_wf_request hwf
+      exact h
+    have hwt_ctx : InstanceOfType Γ env.request.context (.record Γ.reqty.context) := by
+      have ⟨_, ⟨_, _, _, h⟩, _⟩ := hinst
+      exact h
+    have ⟨sym_ctx, hsym_ctx, hsame_sym_ctx⟩ := value_symbolize?_same hwf hwf_ctx_ty hwt_ctx
+    simp only [Value.symbolize?, Option.bind_eq_bind] at hsym_ctx
+    simp only [Option.bind_eq_bind, hsym_ctx]
+    exact hsame_sym_ctx
+
+theorem env_symbolize?_same_entities
+  {Γ : TypeEnv} {env : Env}
+  (hinst : InstanceOfWellFormedEnvironment env.request env.entities Γ) :
+  env.entities ∼ ((SymEnv.ofEnv Γ).interpret (env.symbolize? Γ)).entities
+:= by
+  sorry
+
+theorem env_symbolize?_same
+  {Γ : TypeEnv} {env : Env}
+  (hinst : InstanceOfWellFormedEnvironment env.request env.entities Γ) :
+  env ∼ (SymEnv.ofEnv Γ).interpret (env.symbolize? Γ)
+:= by
+  constructor
+  · exact env_symbolize?_same_request hinst
+  · exact env_symbolize?_same_entities hinst
+
 theorem ofEnv_soundness
   {Γ : TypeEnv} {env : Env}
-  (hmem : InstanceOfWellFormedEnvironment env.request env.entities Γ) :
+  (hinst : InstanceOfWellFormedEnvironment env.request env.entities Γ) :
   env ∈ᵢ SymEnv.ofEnv Γ
-:= sorry
+:= by
+  have ⟨hwf, hinst_req, hinst_sch⟩ := hinst
+  exists env.symbolize? Γ
+  constructor
+  · sorry
+  . exact env_symbolize?_same hinst
 
 end Cedar.Thm
